src/coq/Handlers/MemoryModel.v
@@ -1906,6 +1906,525 @@ Module MakeMemoryModelSpec (LP : LLVMParams) (MP : MemoryParams LP) (MMSP : Memo
   Include MemoryModelSpec LP MP MMSP.
 End MakeMemoryModelSpec.
 
+Module Type MemStateInfinite (LP : LLVMParamsBig) (MP : MemoryParams LP) (MMSP : MemoryModelSpecPrimitives LP MP) (MMS : MemoryModelSpec LP MP MMSP).
+  (* Intptrs are "big" *)
+  Import LP.Events.
+  Import LP.ITOP.
+  Import LP.PTOI.
+  Import LP.IP_BIG.
+  Import LP.IP.
+  Import LP.ADDR.
+  Import LP.PROV.
+
+  Import MMSP.
+  Import MMS.
+  Import MemHelpers.
+
+  Import Monad.
+  Import MapMonadExtra.
+  Import MP.GEP.
+  Import MP.BYTE_IMPL.
+
+  Parameter next_addr : MemState -> (addr * Provenance)%type.
+
+  Parameter next_addr_fresh :
+    forall ms1 ms2 ptr pr,
+      next_addr ms1 = (ptr, pr) ->
+      (* Address is fresh *)
+      (* All previously allocated addresses are smaller *)
+      (forall p aid,
+          addr_allocated_prop p aid (MemState_get_memory ms1) (ret (MemState_get_memory ms1, true)) ->
+          (ptr_to_int ptr > ptr_to_int p)%Z) /\
+        (* Fresh provenance *)
+        address_provenance ptr = allocation_id_to_prov (provenance_to_allocation_id pr) /\
+        (* Provenance not previously used *)
+        ~ used_provenance_prop ms1 pr /\
+        (* Provenance now used *)
+        used_provenance_prop ms2 pr /\
+        (* All provenances preserved... *)
+        (forall pr, used_provenance_prop ms1 pr -> used_provenance_prop ms2 pr).
+        
+  Parameter initialize_memory : MemState -> addr -> Provenance -> list SByte -> MemState.
+
+  Parameter initialize_memory_properties :
+    forall ms1 ptr pr bytes ms2,
+      initialize_memory ms1 ptr pr bytes = ms2 ->
+      (* Provenance is used *)
+      used_provenance_prop ms2 pr.
+
+End MemStateInfinite.
+
+(** Memory models which have unlimited memory *)
+Module MemoryModelInfiniteSpec (LP : LLVMParamsBig) (MP : MemoryParams LP) (MMSP : MemoryModelSpecPrimitives LP MP) (MMS : MemoryModelSpec LP MP MMSP) (MSINF : MemStateInfinite LP MP MMSP MMS).
+  (* Intptrs are "big" *)
+  Import LP.Events.
+  Import LP.ITOP.
+  Import LP.PTOI.
+  Import LP.IP_BIG.
+  Import LP.IP.
+
+  Import MMSP.
+  Import MMS.
+  Import MemHelpers.
+
+  Import MP.GEP.
+
+  Import MSINF.
+  Import Util.
+
+  Import MapMonadExtra.
+  Import Monad.
+
+  Import LP.SIZEOF.
+  Import LP.
+  Import PROV.
+  Import MP.BYTE_IMPL.
+
+  Import DV.
+  (*
+    Things that must succeed:
+
+    - get_consecutive_ptrs: May need something in GepM for this.
+    - byte_allocated: for all of the consecutive pointers
+
+   *)
+
+  (* TODO: Move to something like IP_BIG? *)
+  Lemma big_intptr_seq_succeeds :
+    forall start len,
+    exists ips, intptr_seq start len = NoOom ips.
+  Proof.
+    intros start len.
+    unfold intptr_seq.
+    induction (Zseq start len).
+    - cbn. exists []. reflexivity.
+    - rewrite map_monad_unfold.
+      cbn.
+      break_match.
+      2: {
+        pose proof (from_Z_safe a) as CONTRA.
+        rewrite Heqo in CONTRA.
+        contradiction.
+      }
+
+      destruct IHl as (ips & IHl).
+      exists (i :: ips).
+      Require Import FunctionalExtensionality.
+      setoid_rewrite functional_extensionality.
+      rewrite IHl.
+      reflexivity.
+      reflexivity.
+  Qed.
+
+  #[global] Instance lift_err_RAISE_ERROR_Proper {A M} `{HM: Monad M} `{RAISE: RAISE_ERROR M} `{EQM : Eq1 M} `{EQV : @Eq1Equivalence M HM EQM} :
+    Proper (eq ==> eq1) (@lift_err_RAISE_ERROR A M HM RAISE).
+  Proof.
+    unfold Proper, respectful.
+    intros x y H; subst.
+    reflexivity.
+  Defined.
+
+  Lemma get_consecutive_ptrs_succeeds :
+    forall {M : Type -> Type}
+      `{HM: Monad M} `{EQM : Eq1 M} `{EQV : @Eq1Equivalence M HM EQM}
+      `{EQRET : @Eq1_ret_inv M EQM HM}
+      `{OOM: RAISE_OOM M} `{ERR: RAISE_ERROR M}
+      `{LAWS: @MonadLawsE M EQM HM}
+      ptr len,
+    exists ptrs, (get_consecutive_ptrs ptr len ≈ ret ptrs)%monad.
+  Proof.
+    intros M HM EQM EQV EQRET OOM ERR LAWS ptr len.
+
+    unfold get_consecutive_ptrs.
+    pose proof big_intptr_seq_succeeds 0 len as (ips & SEQ).
+    rewrite SEQ.
+    cbn.
+
+    pose proof map_monad_err_succeeds
+         (fun ix : intptr =>
+            handle_gep_addr (DTYPE_I 8) ptr [LP.Events.DV.DVALUE_IPTR ix])
+         ips as HMAPM.
+
+    forward HMAPM.
+    { intros a IN.
+      eexists.
+      eapply handle_gep_addr_ix'.
+      reflexivity.
+    }
+
+    destruct HMAPM as (res & HMAPM).
+    exists res.
+    rewrite bind_ret_l.
+    rewrite HMAPM.
+    cbn.
+    reflexivity.
+  Qed.
+
+  (* TODO: this can probably more somewhere else *)
+  Lemma get_consecutive_ptrs_cons :
+    forall {M : Type -> Type}
+      `{HM: Monad M} `{EQM : Eq1 M} `{EQV : @Eq1Equivalence M HM EQM}
+      `{EQRET : @Eq1_ret_inv M EQM HM}
+      `{OOM: RAISE_OOM M} `{ERR: RAISE_ERROR M}
+      `{LAWS: @MonadLawsE M EQM HM}
+      ptr len p ptrs,
+      (get_consecutive_ptrs ptr len ≈ ret (p :: ptrs))%monad ->
+      p = ptr /\ (exists ptr' len', get_consecutive_ptrs ptr' len' ≈ ret ptrs)%monad.
+  Proof.
+    intros M HM EQM EQRET EQV OOM ERR LAWS ptr len p ptrs CONSEC.
+
+    unfold get_consecutive_ptrs in *.
+    pose proof big_intptr_seq_succeeds 0 len as (ips & SEQ).
+    rewrite SEQ in *.
+    cbn in *.
+
+    rewrite bind_ret_l in CONSEC.
+    generalize dependent len.
+    induction len; intros SEQ.
+    - cbn in SEQ.
+      inv SEQ.
+      cbn in CONSEC.
+      eapply eq1_ret_ret in CONSEC; [|typeclasses eauto].
+      inv CONSEC.
+    - clear IHlen.
+
+      cbn in *.
+      rewrite from_Z_0 in *.
+      break_match_hyp; inv SEQ.
+
+      cbn in *.
+      rewrite handle_gep_addr_0 in *.
+
+      break_match_hyp.
+      (* TODO: Need some kind of inversion lemma for raise_error and ret *)
+      cbn in *.
+      admit.
+
+      cbn in *.
+      eapply eq1_ret_ret in CONSEC; [|typeclasses eauto].
+      inv CONSEC.
+
+      split; auto.
+      destruct (from_Z 1) as [ix_one | ix_one] eqn:ONE.
+      2: {
+        pose proof from_Z_safe 1 as CONTRA.
+        rewrite ONE in CONTRA.
+        contradiction.
+      }
+
+      destruct (handle_gep_addr (DTYPE_I 8) p [LP.Events.DV.DVALUE_IPTR ix_one]) as [ptr_one | ptr_one] eqn:PTRONE.
+      { erewrite handle_gep_addr_ix' in PTRONE.
+        inv PTRONE.
+        reflexivity.
+      }
+
+      induction len.
+  Admitted.
+
+  (* TODO: this can probably more somewhere else *)
+  Lemma get_consecutive_ptrs_ge :
+    forall {M : Type -> Type}
+      `{HM: Monad M} `{EQM : Eq1 M} `{EQV : @Eq1Equivalence M HM EQM}
+      `{EQRET : @Eq1_ret_inv M EQM HM}
+      `{OOM: RAISE_OOM M} `{ERR: RAISE_ERROR M}
+      `{LAWS: @MonadLawsE M EQM HM}
+      ptr len ptrs,
+      (get_consecutive_ptrs ptr len ≈ ret ptrs)%monad ->
+      (forall p,
+          In p ptrs ->
+          (ptr_to_int ptr <= ptr_to_int p)%Z).
+  Proof.
+    intros M HM EQM EQV EQRET OOM ERR LAWS ptr len ptrs.
+    revert ptr len.
+    induction ptrs; intros ptr len CONSEC p IN.
+    - inv IN.
+    - destruct IN as [IN | IN].
+      + subst.
+        apply get_consecutive_ptrs_cons in CONSEC as (START & CONSEC).
+        subst.
+        lia.
+      + pose proof CONSEC as CONSEC'.
+        apply get_consecutive_ptrs_cons in CONSEC as (START & ptr' & len' & CONSEC).
+        subst.
+        pose proof IHptrs as IHptrs'.
+        specialize (IHptrs' _ _ CONSEC _ IN).
+
+        (* `ptr'` is in `ptrs`, and everything in `ptrs >= ptr'`
+
+           So, I know `ptr' <= p`
+
+           I should know that `ptr < ptr'`...
+         *)
+
+        (* Could take get_consecutive_ptrs in CONSEC and CONSEC' and compare...
+
+           What if ptrs = [ ]?
+
+           I.e., len = 1... Then ptrs is nil and IN is a contradiction.
+        *)
+
+        destruct ptrs as [| ptr'0 ptrs].
+        inv IN.
+
+        (* Need to show that ptr'0 = ptr' *)
+        pose proof CONSEC as CONSEC''.
+        apply get_consecutive_ptrs_cons in CONSEC as (ptreq & ptr'' & len'' & CONSEC).
+        subst.
+
+        assert (ptr_to_int ptr < ptr_to_int ptr')%Z by admit.
+        lia.
+  Admitted.
+
+  Lemma get_consecutive_ptrs_nth :
+    forall {M : Type -> Type}
+      `{HM: Monad M} `{EQM : Eq1 M} `{EQV : @Eq1Equivalence M HM EQM}
+      `{EQRET : @Eq1_ret_inv M EQM HM}
+      `{OOM: RAISE_OOM M} `{ERR: RAISE_ERROR M}
+      `{LAWS: @MonadLawsE M EQM HM}
+      ptr len ptrs,
+      (get_consecutive_ptrs ptr len ≈ ret ptrs)%monad ->
+      (forall p ix_nat,
+          Nth ptrs ix_nat p ->
+          exists ix,
+            NoOom ix = from_Z (Z.of_nat ix_nat) /\
+            handle_gep_addr (DTYPE_I 8) ptr [DVALUE_IPTR ix] = inr p).
+  Proof.
+    intros M HM EQM EQV EQRET OOM ERR LAWS ptr len ptrs CONSEC p ix_nat NTH.
+    pose proof from_Z_safe (Z.of_nat ix_nat) as IX.
+    break_match_hyp; inv IX.
+    rename i into ix.
+    exists ix.
+    split; auto.
+
+    pose proof big_intptr_seq_succeeds 0 len as (ixs & SEQ).
+    unfold get_consecutive_ptrs in *.
+    rewrite SEQ in CONSEC.
+    cbn in CONSEC.
+    rewrite bind_ret_l in CONSEC.
+    cbn in CONSEC.
+    cbn in *.
+
+    pose proof
+         (map_monad_err_Nth
+            (fun ix : intptr => handle_gep_addr (DTYPE_I 8) ptr [DVALUE_IPTR ix])
+            ixs
+            ptrs
+            p
+            ix_nat
+         ) as MAPNTH.
+
+    forward MAPNTH.
+    { destruct (map_monad (fun ix : intptr => handle_gep_addr (DTYPE_I 8) ptr [DVALUE_IPTR ix]) ixs).
+      cbn in CONSEC.
+      (* TODO: Need raise_error inversion lemma *)
+      admit.
+      cbn in CONSEC.
+      eapply eq1_ret_ret in CONSEC; try typeclasses eauto.
+      subst; auto.
+    }
+
+    specialize (MAPNTH NTH).
+    destruct MAPNTH as (ix' & GEP & NTH').
+    cbn in GEP.
+
+    eapply intptr_seq_nth in SEQ; eauto.
+    assert (ix = ix').
+    { cbn in SEQ.
+      rewrite Heqo in SEQ.
+      inv SEQ.
+      auto.
+    }
+
+    subst; auto.
+  Admitted.
+
+  Lemma get_consecutive_ptrs_prov :
+    forall {M : Type -> Type}
+      `{HM: Monad M} `{EQM : Eq1 M} `{EQV : @Eq1Equivalence M HM EQM}
+      `{EQRET : @Eq1_ret_inv M EQM HM}
+      `{OOM: RAISE_OOM M} `{ERR: RAISE_ERROR M}
+      `{LAWS: @MonadLawsE M EQM HM}
+      ptr len ptrs,
+      (get_consecutive_ptrs ptr len ≈ ret ptrs)%monad ->
+      forall p, In p ptrs -> address_provenance p = address_provenance ptr.
+  Proof.
+    intros M HM EQM EQV EQRET OOM ERR LAWS ptr len ptrs CONSEC p IN.
+
+    apply In_nth_error in IN as (ix_nat & NTH).
+    pose proof CONSEC as GEP.
+    eapply get_consecutive_ptrs_nth in GEP; eauto.
+    destruct GEP as (ix & IX & GEP).
+
+    apply handle_gep_addr_preserves_provenance in GEP.
+    auto.
+  Qed.
+
+  Lemma can_find_fresh_block :
+    forall {M : Type -> Type}
+      `{HM: Monad M} `{EQM : Eq1 M} `{EQV : @Eq1Equivalence M HM EQM}
+      `{EQRET : @Eq1_ret_inv M EQM HM}
+      `{OOM: RAISE_OOM M} `{ERR: RAISE_ERROR M}
+      `{LAWS: @MonadLawsE M EQM HM}
+      (m1 : MemState) (m2 : MemState) len,
+    exists pr ptr ptrs,
+      (get_consecutive_ptrs ptr len ≈ ret ptrs)%monad /\
+        (forall p, In p ptrs -> byte_not_allocated m1 p) /\
+        (address_provenance ptr = allocation_id_to_prov (provenance_to_allocation_id pr)) /\
+        (forall p, In p ptrs -> address_provenance p = allocation_id_to_prov (provenance_to_allocation_id pr)) /\
+        ~ used_provenance_prop m1 pr /\
+        used_provenance_prop m2 pr /\
+        (forall pr, used_provenance_prop m1 pr -> used_provenance_prop m2 pr) /\
+        
+  .
+  Proof.
+    intros M HM EQM EQV EQRET OOM ERR LAWS m1 len.
+    set (ptr_w_prov := next_addr m1).
+    set (ptr := fst ptr_w_prov).
+    set (pr := snd ptr_w_prov).
+
+    exists pr.
+    exists ptr.
+    pose proof get_consecutive_ptrs_succeeds ptr len as (ptrs & CONSEC).
+
+    exists ptrs.
+
+    pose proof next_addr_fresh m1 ptr pr as FRESH.
+    forward FRESH.
+    { destruct ptr_w_prov eqn:PTR.
+      auto.
+    }
+
+    destruct FRESH as (FRESH_ADDR & PTR_PROV & FRESH_PROV).
+
+    split; auto.
+    split; auto.
+    { intros p IN.
+
+      unfold byte_not_allocated.
+      intros aid.
+      intros ALLOC.
+      unfold byte_allocated in ALLOC.
+      red in ALLOC.
+
+      specialize (FRESH_ADDR p aid).
+      forward FRESH_ADDR.
+      { cbn in ALLOC.
+        destruct ALLOC as (sab & a & ALLOC & EQ1 & EQ2); subst.
+        unfold lift_memory_MemPropT in ALLOC.
+        destruct ALLOC as (ALLOC & SUCC).
+        cbn in ALLOC.
+        cbn.
+        auto.
+      }
+
+      epose proof (get_consecutive_ptrs_ge _ _ _ CONSEC _ IN).
+      lia.
+    }
+
+    split; auto.
+    split; auto.
+
+    { intros p IN.
+      rewrite <- PTR_PROV.
+      eapply get_consecutive_ptrs_prov; eauto.      
+    }
+  Qed.
+
+  (* Actually, the easy way to do this is to show that the executable version always succeeds...
+
+     Because the executable version is a subset of the allowed behaviours...
+
+     Eh.
+   *)
+  Lemma allocate_can_always_succeed :
+    forall (m1 : MemState) (t : dtyp) (init_bytes : list SByte)
+      (BYTES_SIZE : sizeof_dtyp t = N.of_nat (length init_bytes))
+      (NON_VOID : t <> DTYPE_Void),
+    exists m2 pr ptr ptrs,
+      allocate_bytes_succeeds_spec m1 t init_bytes pr m2 ptr ptrs.
+  Proof.
+    intros m1 t init_bytes BYTES_SIZE NON_VOID.
+
+    epose proof (@can_find_fresh_block (MemPropT MemState) (@MemPropT_Monad MemState) (@MemPropT_Eq1 MemState) _ _ _ _ _ m1 (length init_bytes)) as (pr & ptr & ptrs & CONSEC_PTRS & CONSEC_FRESH & PTR_PR & PTRS_PR & UNUSED_PR).
+    pose proof (big_intptr_seq_succeeds 0 (length init_bytes)) as (ixs & SEQ_ixs).
+
+    (* m1 + init_bytes starting at ptr *)
+    pose proof mem_state_fresh_provenance m1 as (pr' & FRESH_PROV).
+    set (m
+    prov <- fresh_provenance;;
+    set (m2 := initialize_memory m1 ptr pr init_bytes).
+    exists m2.
+    exists pr.
+
+    exists ptr. exists ptrs.
+
+    split.
+    - (* allocate_bytes_consecutive *)
+      apply CONSEC_PTRS.
+      cbn; auto.
+    - (* allocate_bytes_address_provenance *)
+      auto.
+    - (* allocate_bytes_addresses_provenance *)
+      auto.
+    - (* allocate_bytes_provenances_preserved *)
+      intros pr'0.
+      admit.
+    - (* allocate_bytes_was_fresh_byte *)
+      auto.
+    - (* allocate_bytes_now_byte_allocated *)
+      admit.
+    - (* allocate_bytes_preserves_old_allocations *)
+      admit.
+    - (* alloc_bytes_new_reads_allowed *)
+      admit.
+    - (* alloc_bytes_old_reads_allowed *)
+      admit.
+      (* intros ptr' DISJOINT.
+      split; auto. *)
+    - (* alloc_bytes_new_reads *)
+      intros p ix byte NTH1 NTH2.
+      (* apply Util.not_Nth_nil in NTH1. *)
+      (* contradiction. *)
+      admit.
+    - (* alloc_bytes_old_reads *)
+      intros ptr' byte DISJOINT.
+      split; auto.
+      admit.
+      admit.
+    - (* alloc_bytes_new_writes_allowed *)
+      intros p IN.
+      admit.
+      (* inv IN. *)
+    - (* alloc_bytes_old_writes_allowed *)
+      intros ptr' DISJOINT.
+      split; auto.
+      admit.
+      admit.
+    - (* alloc_bytes_add_to_frame *)
+      (*
+      intros fs1 fs2 POP ADD.
+      cbn in ADD; subst; auto.
+      unfold memory_stack_frame_stack_prop in *.
+      cbn in *.
+      unfold memory_stack_frame_stack.
+      cbn.
+      setoid_rewrite add_all_to_frame_nil_preserves_frames.
+      cbn.
+      rewrite POP.
+      auto. *)
+      admit.
+    - (* Heap preserved *)
+      admit.
+      solve_heap_preserved.
+    - (* Non-void *)
+      auto.
+    - (* Length *)
+      cbn; auto.
+*)
+  Admitted.
+
+End MemoryModelInfiniteSpec.
+
 Module Type MemoryExecMonad (LP : LLVMParams) (MP : MemoryParams LP) (MMSP : MemoryModelSpecPrimitives LP MP) (MMS : MemoryModelSpec LP MP MMSP).
   (* TODO: move these imports *)
   Import EitherMonad.
@@ -2382,7 +2901,8 @@ Module MemoryModelTheory (LP : LLVMParams) (MP : MemoryParams LP) (MMEP : Memory
       pose proof (HM ms st VALID) as [[ubm UBM] | NUBM].
       { (* m raised UB *)
         left.
-        repeat eexists; eauto.
+        exists ubm.
+        repeat eexists; cbn; eauto.
       }
 
       (* m did not raise UB *)
